Finish enum validation
The essence of the approach that works is to break things down into many
very small functions, with a handful of generic combinators that are not
unfolded.

examples/kv_parsing/EnumParsing.fst
@@ -5,6 +5,7 @@ open Validator
 open Serializer
 open Slice
 
+open FStar.Seq
 open FStar.HyperStack
 open FStar.HyperStack.ST
 
@@ -34,7 +35,8 @@ let numbers_tag_val n =
   | OneNum _ -> 1uy
   | TwoNums _ _ -> 2uy
 
-let parse_numbers_tag : parser numbers_tag =
+val parse_numbers_tag : parser numbers_tag
+let parse_numbers_tag =
   parse_u8 `and_then`
   (fun t -> if U8.lt t 3uy then parse_ret (t <: numbers_tag) else fail_parser)
 
@@ -50,19 +52,104 @@ let parse_TwoNums : parser (ns:numbers{TwoNums? ns}) =
   (fun n -> parse_u32 `and_then`
   (fun m -> parse_ret #(ns:numbers{TwoNums? ns}) (TwoNums n m)))
 
-let parse_numbers : parser numbers =
-  parse_numbers_tag `and_then`
-  (fun t -> if U8.eq t 0uy
-            then parse_Nothing `and_then` parse_ret
-         else if U8.eq t 1uy
-           then parse_OneNum `and_then` parse_ret
-         else // t == 2uy
-           begin
-            assert (U8.v t == 2);
-            parse_TwoNums `and_then` parse_ret
-           end)
+let parser_forget (#t:Type) (#rf1:t -> Type0) ($p:parser (v:t{rf1 v})) : parser t =
+  fun input -> match p input with
+            | Some (v, off) -> Some (v, off)
+            | None -> None
 
-let parse_numbers_tag_st : parser_st parse_numbers_tag = fun input ->
+let parse_numbers_data (t:numbers_tag) : parser numbers =
+  if U8.eq t 0uy
+    then parser_forget parse_Nothing
+  else if U8.eq t 1uy
+    then parser_forget parse_OneNum
+  else parser_forget parse_TwoNums
+
+let parse_numbers : parser numbers =
+  parse_numbers_tag `and_then` parse_numbers_data
+
+let pure_validator = input:bytes{length input < pow2 32} -> option (off:nat{off <= length input})
+
+let validate_ok (#t:Type) (p: parser t) (v: pure_validator) : Type0 =
+  forall (input: bytes{length input < pow2 32}).
+    match v input with
+    | Some off -> Some? (p input) /\
+                 (let (_, off') = Some?.v (p input) in
+                   off == off')
+    | None -> True
+
+let pure_validator' #t (p: parser t) = v:pure_validator{validate_ok p v}
+
+let parser_forget_ok #t (#rf1:t -> Type0) (p: parser (v:t{rf1 v})) (v: pure_validator) :
+  Lemma (requires (validate_ok p v))
+        (ensures (validate_ok (parser_forget p) v))
+  [SMTPat (validate_ok (parser_forget p) v)] = ()
+
+let make_correct #t (p: parser t) (v:pure_validator) :
+  Pure (pure_validator' p)
+    (requires (validate_ok p v))
+    (ensures (fun r -> True)) = v
+
+let validate_Nothing_pure = make_correct (parser_forget parse_Nothing)
+                            (fun input -> Some 0)
+
+let validate_OneNum_pure = make_correct (parser_forget parse_OneNum)
+                           (fun input -> if length input < 4 then None else Some 4)
+
+let validate_TwoNums_pure = make_correct (parser_forget parse_TwoNums)
+                            (fun input -> if length input < 8 then None else Some 8)
+
+let validate_numbers_data_pure (t:numbers_tag) : pure_validator' (parse_numbers_data t) =
+  make_correct _
+  (if U8.eq t 0uy
+    then validate_Nothing_pure
+  else if U8.eq t 1uy
+    then validate_OneNum_pure
+  else validate_TwoNums_pure)
+
+#reset-options "--z3rlimit 15"
+
+val seq_pure_validate (v1 v2: pure_validator) : pure_validator
+let seq_pure_validate v1 v2 = fun input ->
+  match v1 input with
+  | Some off -> (match v2 (slice input off (length input)) with
+               | Some off' -> Some (off+off')
+               | None -> None)
+  | None -> None
+
+val lemma_seq_pure_validate_A2_ok
+  (#t:Type) (#p: parser t) (v1: pure_validator' p)
+  (#t':Type) (#p': parser t') (v2: pure_validator' p') :
+  Lemma (forall t'' (f: t -> t' -> t'').
+        validate_ok
+          (p `and_then` (fun (v:t) -> p' `and_then` (fun (v':t') -> parse_ret (f v v'))))
+          (seq_pure_validate v1 v2))
+let lemma_seq_pure_validate_A2_ok #t #p v1 #t' #p' v2 = ()
+
+val then_pure_check (#t:Type) (p: parser t) (v: t -> pure_validator) : pure_validator
+let then_pure_check #t p v = fun input ->
+  match p input with
+  | Some (x, off) -> (match v x (slice input off (length input)) with
+                    | Some off' -> Some (off+off')
+                    | None -> None)
+  | None -> None
+
+val lemma_then_pure_check_ok
+  (#t:Type) (#p: parser t)
+  (#t':Type) (#p': t -> parser t') (v: (x:t -> pure_validator' (p' x))) :
+  Lemma (validate_ok
+          (p `and_then` p')
+          (p `then_pure_check` v))
+  [SMTPat (p `then_pure_check` v); SMTPat (p `and_then` p')]
+let lemma_then_pure_check_ok #t #p #t' #p' v = ()
+
+#reset-options
+
+let validate_numbers_pure : pure_validator' parse_numbers =
+  make_correct _
+  (parse_numbers_tag `then_pure_check` validate_numbers_data_pure)
+
+val parse_numbers_tag_st : parser_st parse_numbers_tag
+let parse_numbers_tag_st = fun input ->
   match parse_u8_st input with
   | Some (tag, off) -> if U8.lt tag 3uy
                       then Some ((tag <: numbers_tag), off)
@@ -73,32 +160,74 @@ let parse_numbers_tag_st_nochk : parser_st_nochk parse_numbers_tag = fun input -
   let (tag, off) = parse_u8_st_nochk input in
   ((tag <: numbers_tag), off)
 
+(*
+let validate_numbers (input:bslice) : Stack (option (off:U32.t{U32.v off <= U32.v input.len}))
+  (requires (fun h0 -> live h0 input))
+  (ensures (fun h0 r h1 -> live h1 input /\
+                        modifies_none h0 h1 /\
+                        begin
+                          let bs = as_seq h1 input in
+                          match r with
+                          | Some off -> validate_numbers_pure bs == Some (U32.v off)
+                          | None -> True
+                        end)) =
+  match parse_numbers_tag_st input with
+  | Some (tag, off) ->
+    let input = advance_slice input off in
+    if U8.eq tag 0uy
+      then Some off
+    else (admit(); if U8.eq tag 1uy
+      then if U32.lt input.len 4ul then None else Some (U32.add off 4ul)
+    else begin
+      assert (U8.v tag == 2);
+      if U32.lt input.len 8ul then None else Some (U32.add off 8ul)
+    end)
+  | None -> None
+*)
+
 let check_length (len:U32.t) (input:bslice) : Pure bool
   (requires True)
   (ensures (fun r -> r ==> U32.v input.len >= U32.v len)) = U32.lte len input.len
 
-val validate_OneNum : stateful_validator parse_OneNum
+val validate_OneNum : stateful_validator (parser_forget parse_OneNum)
 let validate_OneNum = fun input ->
   if check_length 4ul input then Some 4ul else None
 
-val validate_TwoNums : stateful_validator parse_TwoNums
+val validate_TwoNums : stateful_validator (parser_forget parse_TwoNums)
 let validate_TwoNums = fun input ->
   if check_length 8ul input then Some 8ul else None
 
-#reset-options "--z3rlimit 10"
+let validate_numbers_data (t:numbers_tag) : stateful_validator (parse_numbers_data t) =
+  if U8.eq t 0uy then
+    (fun input -> Some 0ul) <: stateful_validator (parser_forget parse_Nothing)
+  else if U8.eq t 1uy then
+    validate_OneNum
+  else validate_TwoNums
 
-let validate_numbers : stateful_validator parse_numbers = fun input ->
-  match parse_numbers_tag_st input with
-  | Some (tag, off) -> if U8.eq tag 0uy
-                        then Some off
-                      else if U8.eq tag 1uy
-                        then match validate_OneNum (advance_slice input off) with
-                             | Some off' -> if u32_add_overflows off off' then None else Some (U32.add off off')
-                             | None -> None
-                      else begin
-                             assert (U8.v tag == 2);
-                             match validate_TwoNums (advance_slice input off) with
-                             | Some off' -> if u32_add_overflows off off' then None else Some (U32.add off off')
-                             | None -> None
-                           end
-  | None -> None
+let coerce_validator #t (#p: parser t)
+                        (#p': parser t{forall x. p x == p' x})
+                        (v: stateful_validator p) : stateful_validator p' =
+  fun input -> match v input with
+            | Some off -> Some off
+            | None -> None
+
+#reset-options "--z3rlimit 15"
+
+val and_check (#t:Type) (p: parser t) (p_st: parser_st p)
+              (#t':Type) (#p': t -> parser t') (v: x:t -> stateful_validator (p' x))
+              : stateful_validator (p `and_then` p')
+let and_check #t p p_st #t' #p' v =
+    fun input -> match p_st input with
+              | Some (x, off) ->
+                begin
+                  match v x (advance_slice input off) with
+                  | Some off' -> Some (U32.add off off')
+                  | None -> None
+                end
+              | None -> None
+
+#reset-options
+
+let validate_numbers : stateful_validator parse_numbers =
+    // TODO: parse_numbers_tag is not inferred from the type of parse_numbers_tag_st
+    and_check parse_numbers_tag parse_numbers_tag_st validate_numbers_data
